Align game position datatype and paper presentation

Spectroscopy_Game.thy
@@ -11,16 +11,16 @@ The moves of a weak spectroscopy game depend on the transitions of the processes
 So in other words: If the defender wins the weak spectroscopy game starting with a certain energy, the corresponding behavioural equivalence applies.
 \\ Since we added adding stable and branching conjunctions to a delay bisimulation game, we differentiate the positions accordingly.\<close>
 datatype ('s, 'a) spectroscopy_position =
-         Attacker_Immediate (attacker_state: \<open>'s\<close>) (defender_states: \<open>'s set\<close>) |
-         Attacker_Branch (attacker_state: \<open>'s\<close>) (defender_states: \<open>'s set\<close>) |
-         Attacker_Clause (attacker_state: \<open>'s\<close>) (defender_state: \<open>'s\<close>) |
-         Attacker_Delayed (attacker_state: \<open>'s\<close>) (defender_states: \<open>'s set\<close>) |
-
-         Defender_Branch (attacker_state: \<open>'s\<close>) (attack_action: \<open>'a\<close>)
-                         (attacker_state_succ: \<open>'s\<close>) (defender_states: \<open>'s set\<close>)
-                         (defender_branch_states: \<open>'s set\<close>) |
-         Defender_Conj (attacker_state: \<open>'s\<close>) (defender_states: \<open>'s set\<close>) |
-         Defender_Stable_Conj (attacker_state: \<open>'s\<close>) (defender_states: \<open>'s set\<close>)
+  Attacker_Immediate (attacker_state: \<open>'s\<close>) (defender_states: \<open>'s set\<close>) |
+  Attacker_Delayed (attacker_state: \<open>'s\<close>) (defender_states: \<open>'s set\<close>) |
+  Attacker_Conjunct (attacker_state: \<open>'s\<close>) (defender_state: \<open>'s\<close>) |
+  Attacker_Branch (attacker_state: \<open>'s\<close>) (defender_states: \<open>'s set\<close>) |
+  
+  Defender_Conj (attacker_state: \<open>'s\<close>) (defender_states: \<open>'s set\<close>) |
+  Defender_Stable_Conj (attacker_state: \<open>'s\<close>) (defender_states: \<open>'s set\<close>) |
+  Defender_Branch (attacker_state: \<open>'s\<close>) (attack_action: \<open>'a\<close>)
+                 (attacker_state_succ: \<open>'s\<close>) (defender_states: \<open>'s set\<close>)
+                 (defender_branch_states: \<open>'s set\<close>)
 
 context LTS_Tau begin
 
@@ -50,11 +50,11 @@ fun spectroscopy_moves :: \<open>('s, 'a) spectroscopy_position \<Rightarrow> ('
       = (if p = p' \<and> Q = Q' then Some Some else None)\<close> |
 
   conj_answer:
-    \<open>spectroscopy_moves (Defender_Conj p Q) (Attacker_Clause p' q)
+    \<open>spectroscopy_moves (Defender_Conj p Q) (Attacker_Conjunct p' q)
       = (if p = p' \<and> q \<in> Q then (subtract 0 0 1 0 0 0 0 0) else None)\<close> |
 
   pos_neg_clause:
-    \<open>spectroscopy_moves (Attacker_Clause p q) (Attacker_Delayed p' Q')
+    \<open>spectroscopy_moves (Attacker_Conjunct p q) (Attacker_Delayed p' Q')
       = (if (p = p') then
           (if {q} \<Zsurj>S Q' then Some min1_6 else None)
          else (if ({p} \<Zsurj>S Q'\<and> q=p')
@@ -66,7 +66,7 @@ fun spectroscopy_moves :: \<open>('s, 'a) spectroscopy_position \<Rightarrow> ('
           then Some Some else None)\<close> |
 
   conj_s_answer:
-    \<open>spectroscopy_moves (Defender_Stable_Conj p Q) (Attacker_Clause p' q)
+    \<open>spectroscopy_moves (Defender_Stable_Conj p Q) (Attacker_Conjunct p' q)
       = (if p = p' \<and> q \<in> Q then (subtract 0 0 0 1 0 0 0 0)
          else None)\<close> |
 
@@ -81,7 +81,7 @@ fun spectroscopy_moves :: \<open>('s, 'a) spectroscopy_position \<Rightarrow> ('
          else None)\<close> |
 
   br_answer:
-    \<open>spectroscopy_moves (Defender_Branch p \<alpha> p' Q Q\<alpha>) (Attacker_Clause p'' q)
+    \<open>spectroscopy_moves (Defender_Branch p \<alpha> p' Q Q\<alpha>) (Attacker_Conjunct p'' q)
       = (if (p = p'' \<and> q \<in> Q) then (subtract 0 1 1 0 0 0 0 0) else None)\<close> |
 
   br_obsv:
@@ -98,7 +98,7 @@ fun spectroscopy_moves :: \<open>('s, 'a) spectroscopy_position \<Rightarrow> ('
 fun spectroscopy_defender where
   \<open>spectroscopy_defender (Attacker_Immediate _ _) = False\<close> |
   \<open>spectroscopy_defender (Attacker_Branch _ _) = False\<close> |
-  \<open>spectroscopy_defender (Attacker_Clause _ _) = False\<close> |
+  \<open>spectroscopy_defender (Attacker_Conjunct _ _) = False\<close> |
   \<open>spectroscopy_defender (Attacker_Delayed _ _) = False\<close> |
   \<open>spectroscopy_defender (Defender_Branch _ _ _ _ _) = True\<close> |
   \<open>spectroscopy_defender (Defender_Conj _ _) = True\<close> |
@@ -128,12 +128,12 @@ next
     show ?thesis
       by (cases g', simp_all, (smt (z3) option.distinct(1) option.sel minus_component_leq)+)
   next
-    case (Attacker_Clause p q)
+    case (Attacker_Conjunct p q)
     hence \<open>\<exists>p' Q'. g'= (Attacker_Delayed p' Q')\<close>
       using monotonicity_assms(1,2)
-      by (metis spectroscopy_defender.cases spectroscopy_moves.simps(22,23,26,46,62,67))
+      by (induct, auto)
     hence \<open>spectroscopy_moves g g' = Some min1_6 \<or> spectroscopy_moves g g' = Some (\<lambda>e. Option.bind ((subtract_fn 0 0 0 0 0 0 0 1) e) min1_7)\<close>
-      using monotonicity_assms(1,2) Attacker_Clause
+      using monotonicity_assms(1,2) Attacker_Conjunct
       by (smt (verit, ccfv_threshold) spectroscopy_moves.simps(7))
     thus ?thesis
     proof safe
@@ -156,7 +156,8 @@ next
       (\<exists>p' Q'. g'=(Defender_Conj p' Q')) \<or>
       (\<exists>p' Q'. g'=(Defender_Stable_Conj p' Q')) \<or>
       (\<exists>p' p'' Q' \<alpha> Q\<alpha> . g'= (Defender_Branch p' \<alpha> p'' Q' Q\<alpha>))\<close>
-      by (metis monotonicity_assms(1) spectroscopy_defender.cases spectroscopy_moves.simps(27,59))
+      using monotonicity_assms(1)
+      by (induct, auto)
     thus ?thesis
     proof (safe)
       fix p' Q'
@@ -226,12 +227,11 @@ next
       by (cases g', auto)
         (smt (verit, best) option.distinct(1) option.inject order.trans)+
   next
-    case (Attacker_Clause p q)
+    case (Attacker_Conjunct p q)
     hence \<open>\<exists>p' Q'. g'= (Attacker_Delayed p' Q')\<close>
-      using defender_win_min_assms(2)
-      by (metis spectroscopy_defender.cases spectroscopy_moves.simps(21,52,58,62,67,72))
+      using defender_win_min_assms(2) by (induct, auto)
     hence \<open>spectroscopy_moves g g' = Some min1_6 \<or> spectroscopy_moves g g' = Some (\<lambda>e. Option.bind ((subtract_fn 0 0 0 0 0 0 0 1) e) min1_7)\<close>
-      using defender_win_min_assms(2) Attacker_Clause
+      using defender_win_min_assms(2) Attacker_Conjunct
       by (smt (verit, ccfv_threshold) spectroscopy_moves.simps(7))
     thus ?thesis
     proof safe
@@ -251,7 +251,7 @@ next
       (\<exists>p' Q'. g'=(Defender_Conj p' Q')) \<or>
       (\<exists>p' Q'. g'=(Defender_Stable_Conj p' Q')) \<or>
       (\<exists>p' p'' Q' \<alpha> Q\<alpha> . g'= (Defender_Branch p' \<alpha> p'' Q' Q\<alpha>))\<close>
-      by (metis defender_win_min_assms(2) spectroscopy_defender.cases spectroscopy_moves.simps(27,59))
+      using defender_win_min_assms(2) by (induct, auto)
     thus ?thesis
     proof (safe)
       fix p' Q'
@@ -294,7 +294,7 @@ next
     qed
   next
     case (Defender_Branch p a p' Q' Qa)
-    hence \<open>(\<exists>q'\<in>Q'. g' = Attacker_Clause p q')
+    hence \<open>(\<exists>q'\<in>Q'. g' = Attacker_Conjunct p q')
       \<or> (\<exists>Qa'. Qa \<mapsto>aS a Qa' \<and> g' = Attacker_Branch p' Qa')\<close>
       using defender_win_min_assms by (cases g', auto) (metis not_None_eq)+
     hence \<open>(spectroscopy_moves g g') = (subtract 0 1 1 0 0 0 0 0) \<or>
