Silent_Step_Spectroscopy.thy
@@ -9,20 +9,19 @@ begin
 context weak_spectroscopy_game
 begin
 
-text \<open>\label{th1}\<close>
-
 theorem spectroscopy_game_correctness:
   fixes e p Q
   shows \<open>(\<exists>\<phi>. distinguishes_from \<phi> p Q \<and> expressiveness_price \<phi> \<le> e)
        = (attacker_wins e (Attacker_Immediate p Q))\<close>
 proof
   assume \<open>\<exists>\<phi>. distinguishes_from \<phi> p Q \<and> expressiveness_price \<phi> \<le> e\<close>
-  then obtain \<phi> where
-    \<open>distinguishes_from \<phi> p Q\<close> and le: \<open>expressiveness_price \<phi> \<le> e\<close>
+  then obtain \<phi> where \<phi>_spec:
+    \<open>distinguishes_from \<phi> p Q\<close> \<open>expressiveness_price \<phi> \<le> e\<close>
     unfolding \<O>_def by blast
-  from distinction_implies_winning_budgets this(1)
-    have budget: \<open>attacker_wins (expressiveness_price \<phi>) (Attacker_Immediate p Q)\<close> .
-  thus \<open>attacker_wins e (Attacker_Immediate p Q)\<close> using win_a_upwards_closure le by simp
+  from distinction_implies_winning_budgets \<phi>_spec(1) have
+    \<open>attacker_wins (expressiveness_price \<phi>) (Attacker_Immediate p Q)\<close> .
+  thus \<open>attacker_wins e (Attacker_Immediate p Q)\<close>
+    using win_a_upwards_closure \<phi>_spec(2) by simp
 next
   assume \<open>attacker_wins e (Attacker_Immediate p Q)\<close>
   with winning_budget_implies_strategy_formula have
